grammatik/Grammatik.lean
@@ -210,3 +210,6 @@ import Grammatik.Schlusssatz104
 import Grammatik.Korrespondenz
 import Grammatik.Gleitkomma
 import Grammatik.GleitZeuge
+import Grammatik.GleitkommaBits
+import Grammatik.CFormenF
+import Grammatik.CFormenFZeuge
